Move simultaneous substitutions to their own file

theories/unification/Unification.v
@@ -43,7 +43,7 @@ From Equations.Type Require
 From Equations.Prop Require
      Classes.
 From Em Require Import
-     Definitions Context Environment Prelude STLC Triangular.
+     Definitions Context Environment Prelude STLC Triangular Substitution.
 Import ctx.
 Import ctx.notations.
 Import SigTNotations.
@@ -56,7 +56,6 @@ Set Implicit Arguments.
 #[local] Open Scope indexed_scope.
 
 Reserved Notation "w1 ⊒ w2" (at level 80).
-Reserved Notation "w1 ⊒ˢ w2" (at level 80).
 
 Definition Box (A : TYPE) : TYPE :=
   fun w0 => forall w1, w0 ⊒⁻ w1 -> A w1.
@@ -70,10 +69,6 @@ Notation "◇ A" := (DiamondT id A) (at level 9, format "◇ A", right associati
 Notation "? A" := (Option A) (at level 9, format "? A", right associativity).
 Notation "◆ A" := (DiamondT Option A) (at level 9, format "◆ A", right associativity).
 Notation "A * B" := (Prod A B).
-
-Notation "'∀' x .. y , P " :=
-  (Forall (fun x => .. (Forall (fun y => P)) ..))
-    (at level 99, x binder, y binder, right associativity).
 
 Section Löb.
 
@@ -151,179 +146,6 @@ Definition η1 {A} {w x} {xIn : x ∈ w} (t : Ty (w - x)) (a : A (w - x)) : ◆A
 (*   induction t; cbn; f_equal; auto. unfold thickIn. *)
 (*   now rewrite occurs_check_view_thin. *)
 (* Qed. *)
-
-Module Sub.
-
-  Definition Sub (w1 w2 : World) : Type :=
-    @env.Env nat (fun _ => Ty w2) w1.
-  Local Notation "w1 ⊒ˢ w2" := (Sub w1 w2).
-
-  Definition Box (A : TYPE) : TYPE :=
-    fun w0 => forall w1, w0 ⊒ˢ w1 -> A w1.
-  Local Notation "□ A" := (Box A) (at level 9, format "□ A", right associativity).
-
-  Definition subst : ⊢ Ty -> □Ty :=
-    fun w1 =>
-      fix subst (S : Ty w1) {w2} (ζ : w1 ⊒ˢ w2) {struct S} : Ty w2 :=
-      match S with
-      | Ty_hole σIn   => env.lookup ζ σIn
-      | Ty_bool       => Ty_bool
-      | Ty_func S1 S2 => Ty_func (subst S1 ζ) (subst S2 ζ)
-      end.
-
-  Definition id {w} : w ⊒ˢ w :=
-    env.tabulate (fun _ => Ty_hole).
-  Definition thick {w x} (xIn : x ∈ w) (s : Ty (w - x)) : w ⊒ˢ w - x :=
-    env.tabulate (thickIn xIn s).
-  Definition thin {w x} (xIn : x ∈ w) : w - x ⊒ˢ w :=
-    env.tabulate (fun y yIn => Ty_hole (in_thin xIn yIn)).
-  Definition comp {w0 w1 w2} (ζ1 : w0 ⊒ˢ w1) (ζ2 : w1 ⊒ˢ w2) : w0 ⊒ˢ w2 :=
-    env.map (fun _ t => subst t ζ2) ζ1.
-  Local Infix "⊙ˢ" := comp (at level 60, right associativity).
-
-  Fixpoint triangular {w1 w2} (ζ : w1 ⊒⁻ w2) : w1 ⊒ˢ w2 :=
-    match ζ with
-    | Tri.refl       => id
-    | Tri.cons x t ζ => comp (thick _ t) (triangular ζ)
-    end.
-
-  Lemma lookup_id {w x} (xIn : x ∈ w)  :
-    env.lookup id xIn = Ty_hole xIn.
-  Proof. unfold id. now rewrite env.lookup_tabulate. Qed.
-
-  Lemma lookup_comp {w1 w2 w3 x} (xIn : x ∈ w1) (ζ1 : w1 ⊒ˢ w2) (ζ2 : w2 ⊒ˢ w3) :
-    env.lookup (comp ζ1 ζ2) xIn = subst (env.lookup ζ1 xIn) ζ2.
-  Proof. unfold comp. now rewrite env.lookup_map. Qed.
-
-  Lemma lookup_thin {w x y} (xIn : x ∈ w) (yIn : y ∈ w - x) :
-    env.lookup (thin xIn) yIn = Ty_hole (in_thin xIn yIn).
-  Proof. unfold thin. now rewrite env.lookup_tabulate. Qed.
-
-  Lemma lookup_thick {w x y} (xIn : x ∈ w) (t : Ty _) (yIn : y ∈ w) :
-    env.lookup (thick xIn t) yIn = thickIn xIn t yIn.
-  Proof. unfold thick. now rewrite env.lookup_tabulate. Qed.
-
-  Lemma subst_id {w} (t : Ty w) :
-    subst t id = t.
-  Proof. induction t; cbn; f_equal; now rewrite ?lookup_id. Qed.
-
-  Lemma subst_comp {w1} (t : Ty w1) {w2 w3} (ζ2 : w2 ⊒ˢ w3) (ζ1 : w1 ⊒ˢ w2) :
-    subst t (comp ζ1 ζ2) = subst (subst t ζ1) ζ2.
-  Proof. induction t; cbn; f_equal; now rewrite ?lookup_comp. Qed.
-
-  Lemma comp_assoc {w1 w2 w3 w4} (ζ1 : w1 ⊒ˢ w2) (ζ2 : w2 ⊒ˢ w3) (ζ3 : w3 ⊒ˢ w4) :
-    comp (comp ζ1 ζ2) ζ3 = comp ζ1 (comp ζ2 ζ3).
-  Proof.
-    apply env.lookup_extensional. intros x xIn.
-    now rewrite ?lookup_comp, subst_comp.
-  Qed.
-
-  Lemma comp_id_left {w1 w2} (ζ : w1 ⊒ˢ w2) : comp id ζ = ζ.
-  Proof.
-    apply env.lookup_extensional. intros x xIn.
-    now rewrite lookup_comp, lookup_id.
-  Qed.
-
-  Lemma comp_id_right {w1 w2} (ζ : w1 ⊒ˢ w2) :
-    comp ζ id = ζ.
-  Proof.
-    apply env.lookup_extensional. intros x xIn.
-    now rewrite lookup_comp, subst_id.
-  Qed.
-
-  Lemma triangular_trans {w0 w1 w2} (ζ01 : w0 ⊒⁻ w1) (ζ12 : w1 ⊒⁻ w2) :
-    triangular (Tri.trans ζ01 ζ12) =
-      comp (triangular ζ01) (triangular ζ12).
-  Proof.
-    induction ζ01; cbn [triangular Tri.trans].
-    - now rewrite comp_id_left.
-    - now rewrite comp_assoc, IHζ01.
-  Qed.
-
-  Lemma comp_thin_thick {w x} (xIn : x ∈ w) (t : Ty (w - x)) :
-    comp (thin xIn) (thick xIn t) = id.
-  Proof.
-    apply env.lookup_extensional. intros y yIn.
-    rewrite lookup_comp, lookup_id, lookup_thin. cbn.
-    rewrite lookup_thick. unfold thickIn.
-    now rewrite occurs_check_view_thin.
-  Qed.
-
-  Lemma subst_thin {w x} (xIn : x ∈ w) (T : Ty (w - x)) :
-    Triangular.thin xIn T = subst T (thin xIn).
-  Proof. induction T; cbn; f_equal; now rewrite ?lookup_thin. Qed.
-
-  Definition geq {w0 w1} (ζ1 : w0 ⊒ˢ w1) [w2] (ζ2 : w0 ⊒ˢ w2) : Prop :=
-    exists ζ12 : w1 ⊒ˢ w2, ζ2 = ζ1 ⊙ˢ ζ12.
-  Notation "ζ1 ≽ ζ2" := (geq ζ1 ζ2) (at level 80).
-
-  Lemma geq_refl {w1 w2} (ζ : w1 ⊒ˢ w2) : ζ ≽ ζ.
-  Proof. exists Sub.id. symmetry. apply Sub.comp_id_right. Qed.
-
-  Lemma geq_trans {w0 w1 w2 w3} (ζ1 : w0 ⊒ˢ w1) (ζ2 : w0 ⊒ˢ w2) (ζ3 : w0 ⊒ˢ w3) :
-    ζ1 ≽ ζ2 -> ζ2 ≽ ζ3 -> ζ1 ≽ ζ3.
-  Proof.
-    intros [ζ12 H12] [ζ23 H23]. rewrite H23, H12.
-    exists (ζ12 ⊙ˢ ζ23). apply Sub.comp_assoc.
-  Qed.
-
-  Lemma geq_precom {w0 w1 w2 w3} (ζ1 : w0 ⊒ˢ w1) (ζ2 : w1 ⊒ˢ w2) (ζ3 : w1 ⊒ˢ w3) :
-    ζ2 ≽ ζ3 -> ζ1 ⊙ˢ ζ2 ≽ ζ1 ⊙ˢ ζ3.
-  Proof. intros [ζ23 ->]. exists ζ23. symmetry. apply Sub.comp_assoc. Qed.
-
-  Lemma geq_max {w1 w2} (ζ : w1 ⊒ˢ w2) : id ≽ ζ.
-  Proof. exists ζ. symmetry. apply Sub.comp_id_left. Qed.
-
-  Lemma geq_extend {w0 w1 w2} (ζ1 : w0 ⊒ˢ w1) (ζ2 : w1 ⊒ˢ w2) : ζ1 ≽ ζ1 ⊙ˢ ζ2.
-  Proof. now exists ζ2. Qed.
-
-  Fixpoint geqb {w0 w1} (ζ1 : w0 ⊒⁻ w1) [w2] (ζ2 : w0 ⊒ˢ w2) {struct ζ1} : bool :=
-    match ζ1 with
-    | Tri.refl => true
-    | Tri.cons x t ζ1 =>
-        let ζ2' := thin _ ⊙ˢ ζ2 in
-        if Ty_eqdec (subst (Ty_hole _) ζ2) (subst t ζ2')
-        then geqb ζ1 ζ2'
-        else false
-    end.
-  Infix "≽?" := geqb (at level 80).
-
-  Lemma geqb_spec {w0 w1} (ζ1 : w0 ⊒⁻ w1) :
-    forall [w2] (ζ2 : w0 ⊒ˢ w2),
-      Bool.reflect (triangular ζ1 ≽ ζ2) (ζ1 ≽? ζ2).
-  Proof.
-    induction ζ1; cbn [geqb triangular]; intros w2 ζ2.
-    - constructor. apply geq_max.
-    - destruct Ty_eqdec.
-      + destruct (IHζ1 _ (thin xIn ⊙ˢ ζ2)); constructor; clear IHζ1.
-        * destruct g as [ζ2']. exists ζ2'.
-          rewrite comp_assoc. rewrite <- H. clear - e.
-          apply env.lookup_extensional.
-          intros y yIn.
-          rewrite lookup_comp.
-          rewrite lookup_thick. unfold thickIn.
-          destruct (occurs_check_view xIn yIn). apply e.
-          cbn. rewrite lookup_comp. unfold thin.
-          now rewrite env.lookup_tabulate.
-        * intros [ζ2' ->]. apply n. clear n. exists ζ2'.
-          rewrite <- ?comp_assoc.
-          rewrite comp_thin_thick.
-          rewrite comp_id_left.
-          reflexivity.
-      + constructor. intros [ζ2' ->]. apply n. clear n.
-        rewrite <- ?comp_assoc.
-        rewrite comp_thin_thick.
-        rewrite comp_id_left.
-        cbn. rewrite ?lookup_comp, lookup_thick.
-        unfold thickIn. rewrite occurs_check_view_refl.
-        now rewrite subst_comp.
-  Qed.
-
-End Sub.
-Infix "⊒ˢ" := Sub.Sub.
-Infix "⊙ˢ" := Sub.comp (at level 60, right associativity).
-Infix "≽ˢ" := Sub.geq (at level 80).
-(* Infix "≽?" := Sub.geqb (at level 80). *)
 
 (* Infix "≽⁻" := Tri.geq (at level 80). *)
 (* Infix "≽?" := Sub.geqb (at level 80). *)
